\input{preamble.tex}
\input{definitions.tex}


\everymath{\displaystyle}
\pagestyle{askhseis}

\begin{document}


\begin{center}
  \minibox{\large \bfseries \textcolor{Col1}{Αναπτύγματα Βασικών Συναρτήσεων}}
\end{center}

\vspace{\baselineskip}

\setlength{\jot}{10pt}
\begin{align*}
\color{Col1}{\frac{1}{1-x}}&= 1+x+x^2+\cdots +x^n+\cdots = \sum_{n=0}^{\infty}x^n, \quad \text{για}\; \abs{x}<1 \\
\color{Col1}\frac{1}{1+x}&=1-x+x^2-\cdots+(-1)^nx^n+\cdots = \sum_{n=0}^{\infty}(-1)^n x^n, \quad \text{για}\; \abs{x}<1 \\
\color{Col1}e^x&= 1+x+\frac{x^2}{2!}+\cdots+\frac{x^n}{n!}+\cdots = \sum_{n=0}^{\infty}\frac{x^n}{n!}, \quad \text{για}\; \abs{x}<\infty \\
\color{Col1}\sin x&=x-\frac{x^3}{3!}+\frac{x^5}{5!}-\cdots+\frac{(-1)^n x^{2n+1}}{(2n+1)!}+\cdots = \sum_{n=0}^{\infty}\frac{(-1)^nx^{2n+1}}{(2n+1)!},\quad \text{για}\; \abs{x}<\infty \\
\color{Col1}\cos x&=1-\frac{x^2}{2!}+\frac{x^4}{4!}-\cdots \frac{(-1)^nx^{2n}}{(2n)!}+\cdots = \sum_{n=0}^{\infty}\frac{(-1)^nx^{2n}}{(2n)!}, \quad \text{για}\; \abs{x}<\infty \\
\color{Col1}\ln(1+x)&=x-\frac{x^2}{2}+\frac{x^3}{3}-\cdots+\frac{(-1)^{n+1}x^n}{n}+\cdots=\sum_{n=1}^{\infty}\frac{(-1)^{n+1}x^n}{n}, \quad \text{για}\; -1<x\leq 1 \\
\color{Col1}-\ln(1-x)&=x+\frac{x^2}{2}+\frac{x^3}{3}+\cdots+\frac{x^n}{n}+\cdots = \sum_{n=1}^{\infty}\frac{x^n}{n}, \quad \text{για}\; -1\leq x<1 \\
\color{Col1}\arctan x&=x-\frac{x^3}{3}+\frac{x^5}{5}-\cdots+\frac{(-1)^nx^{2n+1}}{2n+1}+\cdots = \sum_{n=0}^{\infty}\frac{(-1)^nx^{2n+1}}{2n+1},\quad \text{για}\; \abs{x}\leq 1 \\
\color{Col1}\sinh x&= x +\frac{x^3}{3!}+\frac{x^5}{5!}+\cdots+\frac{x^{2n+1}}{(2n+1)!}+\cdots = \sum_{n=0}^{\infty}\frac{x^{2n+1}}{(2n+1)!},\quad \text{για}\; \abs{x}<\infty \\
\color{Col1}\cosh x&= 1+\frac{x^2}{2!}+\frac{x^4}{4!}+\cdots +\frac{x^{2n}}{(2n)!}+\cdots = \sum_{n=0}^{\infty}\frac{x^{2n}}{(2n)!}, \quad \text{για}\; \abs{x}<\infty
\end{align*}




\end{document}
