\input{preamble_ask.tex}
\input{definitions_ask.tex}

\pagestyle{askhseis}

\geometry{left=18mm,right=18mm,top=30.00mm,bottom=36.00mm,footskip=24.16mm,headsep=24.16mm}
\everymath{\displaystyle}

\begin{document}

\begin{center}
  \minibox{\large\bfseries \textcolor{Col1}{Μετασχηματισμός Laplace}}
\end{center}

\vspace{\baselineskip}

\twocolumnsides{
\section*{Laplace βασικών συναρτήσεων}
  \begin{enumerate}
    \item $ \mathcal{L}\{1\} = \frac{1}{s}$
    \item $ \mathcal{L}\{t\} = \frac{1}{s^{2}}$
    \item $ \bm{\mathcal{L}\{t^{n}\} = \frac{n!}{s^{n+1}}}$
      \begin{enumerate}[label=\roman*),labelindent=0pt]
        \item $ \mathcal{L}\{t^{2}\} = \frac{2}{s^{3}}$
        \item $ \mathcal{L}\{t^{3}\} = \frac{6}{s^{4}}$
      \end{enumerate}
    \item $ \mathcal{L}\{\mathrm{e}^{at}\} = \frac{1}{s-a}$
    \item $ \mathcal{L}\{\sin{bt}\} = \frac{b}{s^{2}+b^{2}}$
    \item $ \mathcal{L}\{\cos{bt}\} = \frac{s}{s^{2}+b^{2}}$
    \item $ \mathcal{L}\{\sinh{bt}\} = \frac{b}{s^{2}-b^{2}}$
    \item $ \mathcal{L}\{\cosh{bt}\} = \frac{s}{s^{2}-b^{2}}$
    \item $ \bm{\mathcal{L}\{e^{at}f(t)\} = F(s-a)}$
  \end{enumerate}
  \begin{enumerate}[label=\roman*),leftmargin=*,labelindent=20pt]
    \item $ \mathcal{L}\left\{t^{n} \mathrm{e}^{at}\right\} = \frac{n!}{(s-a)^{n+1}} $
    \item $ \mathcal{L}\{e^{at} \sin{bt}\} = \frac{b}{(s-a)^{2}+b^{2}}$
    \item $ \mathcal{L}\{e^{at} \cos{bt}\} = \frac{s-a}{(s-a)^{2}+b^{2}}$
    \item $ \mathcal{L}\{e^{at} \sinh{bt}\} = \frac{b}{(s-a)^{2}-b^{2}}$
    \item $ \mathcal{L}\{e^{at} \cosh{bt}\} = \frac{s-a}{(s-a)^{2}-b^{2}}$
  \end{enumerate}
  }{
  \section*{Ιδιότητες}
  \begin{enumerate}
    \item $ \mathcal{L}\left\{t^{a}\right\} = \frac{\Gamma{(a+1)}}{s^{a+1}}, \quad a>-1 $
    \item $ \mathcal{L}\{tf(t)\} = -F'(s) $
    \item $ \mathcal{L}\{t^{n}f(t)\} = (-1)^{n} F^{(n)}(s) $
      \begin{enumerate}[i)]
        \item $ \mathcal{L}\left\{ty'\right\} = -sY'(s)-Y(s) $ 
        \item $ \mathcal{L}\left\{ty''\right\} = -s^{2}Y'(s)-2Y'(s)+y(0) $ 
      \end{enumerate}
    \item $ \mathcal{L}\{u(t)\} = {1}/{s}$
    \item $ \mathcal{L}\{u_{a}(t)\} = \frac{\mathrm{e}^{-as}}{s}$
    \item $ \bm{\mathcal{L}\{u_{a}(t)f(t-a)\} = \mathrm{e}^{-as}F(s)}$
    \item $ \mathcal{L}\{\delta(t)\} = 1 $
    \item $ \mathcal{L}\{\delta(t-a)\} = \mathrm{e}^{-as} $
    \item $ \mathcal{L}\{f(at)\} = \frac{1}{a} F\left(\frac{s}{a}\right) $
    \item $ \mathcal{L}\left\{\frac{f(t)}{t} \right\} = \int\nolimits _{s}^{\infty} 
      F(\tau) \,{d\tau} $
    \item $ \mathcal{L}\left\{\int\nolimits _{0}^{t} f(\tau) \,{d\tau}\right\} = 
      \frac{F(s)}{s} $
  \end{enumerate}

  \section*{Συνάρτηση Γάμμα}
  \[
    \boxed{\Gamma (t) = \int _{0}^{\infty} \mathrm{e}^{-x} x^{t-1} \,{dx}}
  \] 
  \begin{myitemize}
    \item $\Gamma (t+1) = t \cdot \Gamma (t), \quad t \in \mathbb{R} $
    \item $\Gamma (n+1) = n \cdot \Gamma (n) = n!, \quad n \in \mathbb{N}$
    \item $\Gamma \left(\frac{1}{2}\right) = \sqrt{\pi}$
  \end{myitemize}
}

\section*{Χρήσιμες Σχέσεις}
\centering
\begin{myitemize}
  \item $ \mathcal{L}\{y'(t)\} = sY(s) - y(0) $
  \item $ \mathcal{L}\{y''(t)\} = s^{2}Y(s) - sy(0) - y'(0) $
  \item $ \mathcal{L}\{y'''(t)\} = s^{3}Y(s) - s^{2}y(0) - sy'(0) - y''(0) $
  \item $ \mathcal{L}\{f^{(n)}(t)\} = s^{n} F(s) - s^{n-1}f(0) - s^{n-2}f'(0) - 
    \cdots - sf^{(n-2)}(0)- f^{(n-1)}(0) $
\end{myitemize}


\end{document}
