\begin{example}
  $ \lim_{x \to \infty} \frac{\ln{x}}{x^{2}+1}
  \overset{\left(\frac{0}{0}\right)}{\underset{\mathrm{LH}}{=}} \lim_{x \to
  \infty} \frac{\frac{1}{x}}{2x} = \lim_{x \to \infty} \frac{1}{2x^{2}}
  \overset{\left(\frac{1}{\infty}\right)}{=} 0 $ 
\end{example}

\begin{example}
  $ \lim_{x \to 0} \frac{\arctan{x}}{2x}
  \overset{\left(\frac{0}{0}\right)}{\underset{\mathrm{LH}}{=}} \lim_{x \to 0}
  \frac{\frac{1}{1+x^{2}}}{2} = \lim_{x \to 0} \frac{1}{2(1+x^{2})} = \frac{1}{2}
  $ 
\end{example}

\begin{example}
  $ \lim_{x \to 0} \frac{\mathrm{e}^{x^{2}} -1}{1- \cos{x}}
  \overset{\left(\frac{0}{0}\right)}{\underset{\mathrm{LH}}{=}} \lim_{x \to 0}
  \frac{2x \mathrm{e}^{x^{2}}}{\sin{x}} =
  \overset{\left(\frac{0}{0}\right)}{\underset{\mathrm{LH}}{=}} \lim_{x \to 0}
  \frac{2 \mathrm{e}^{x^{2}}+4x^{2} \mathrm{e}^{x^{2}}}{\cos{x}} = 2 $  
\end{example}

\begin{example}
  $ \lim_{x \to 0^{+}} x^{2} \ln{x} \overset{(0\cdot \infty)}{=} \lim_{x \to 0^{+}} 
  \frac{\ln{x}}{\frac{1}{x^{2}}}
  \overset{\left(\frac{0}{0}\right)}{\underset{\mathrm{LH}}{=}}
  \lim_{x \to 0^{+}} \frac{\frac{1}{x}
  }{- \frac{2}{x^{3}}} = \lim_{x \to 0^{+}} \left(-\frac{x^{2}}{2}\right) = 0 $
\end{example}

\begin{example}
  $ \lim_{x \to \pm \infty} x \sin{\frac{1}{x}} \overset{(0\cdot \infty)}{=}
  \lim_{x \to \pm \infty} \frac{\sin{\frac{1}{ x}}}{\frac{1}{x}}
  \overset{\left(\frac{0}{0}\right)}{\underset{\mathrm{LH}}{=}} \lim_{x \to \pm
  \infty} \frac{\cos{\frac{1}{x}} \cdot (- \frac{1}{x^{2}})}{- \frac{1}{x^{2}}} =
  \lim_{x \to \pm \infty} \cos{x} = 1 $
\end{example}

\begin{example}
  \begin{align*}
    \lim_{x \to \infty} (\ln{x} - \sqrt{x}) \overset{(\infty- \infty)}{=} \lim_{x \to
    \infty} \sqrt{x} \left(\frac{\ln{x}}{\sqrt{x}}-1\right) = 
    \lim_{x \to \infty} \sqrt{x} \cdot
    \lim_{x \to \infty} \left(\frac{\ln{x}}{\sqrt{x}} - 1\right)
  \end{align*}
  \begin{myitemize}
    \item $ \lim_{x \to \infty} \sqrt{x} = \infty $
    \item $ \lim_{x \to \infty} \frac{\ln{x}}{\sqrt{x}}
      \overset{\left(\frac{0}{0}\right)}{\underset{\mathrm{LH}}{=}} \lim_{x \to \infty}
      \frac{\frac{1}{x}}{\frac{1}{2 \sqrt{x}}} = \lim_{x \to \infty}
      \frac{2}{\sqrt{x}} = 0 $
  \end{myitemize}
  Άρα 
  $ \lim_{x \to \infty} \sqrt{x} \cdot \lim_{x \to \infty}
  \left(\frac{\ln{x}}{\sqrt{x}} -1\right) = \infty\cdot (0-1) = - \infty $
\end{example}

\begin{example}
  \begin{align*}
    \lim_{x \to 1} (\frac{x}{x-1} - \frac{1}{\ln{x}}) 
    &= \overset{(\infty- \infty)}{=}
    \lim_{x \to 1} \frac{x \ln{x} - (x-1)}{(x-1) \ln{x}}
    \overset{\left(\frac{0}{0}\right)}{\underset{\mathrm{LH}}{=}} \lim_{x \to 1}
    \frac{\ln{x} + \frac{1}{x} \cdot x -1}{\ln{x} + (x-1) \frac{1}{x}} \\
    &= \lim_{x \to 1} \frac{x \ln{x}}{x \ln{x} +(x-1)}
    \overset{\left(\frac{0}{0}\right)}{\underset{\mathrm{LH}}{=}} \lim_{x \to 1}
    \frac{\ln{x} +1}{\ln{x} +2} = \frac{1}{2}
  \end{align*}
  \end{example}
	


