\begin{exercises}
\item {}
    \begin{enumerate}
        \item Να δείξετε ότι $ - ( \mathbf{u}+ \mathbf{v} ) = - \mathbf{u} - 
            \mathbf{v} $.
        \item Αν $ \lambda \in \mathbb{K}, \; \lambda \neq 0 $ και 
            $ \lambda \cdot \mathbf{u}= \lambda \cdot \mathbf{v}$, τότε να 
            δείξετε ότι $ \mathbf{u} = \mathbf{v} $.
        \item Αν $ \lambda_{1}, \; \lambda _{2} \in \mathbb{K} $ και 
            $ \mathbf{u} \in V, \; \mathbf{u} \neq \mathbf{0} $ με 
            $ \lambda _{1}\cdot \mathbf{u} = \lambda _{2} \cdot \mathbf{u}$, 
            τότε να δείξετε ότι $ \lambda _{1} = \lambda _{2} $.
    \end{enumerate}
\end{exercises}
